checkpoint

Vizing/Path/Defs.lean
@@ -15,6 +15,10 @@ variable {c n : Nat} {G : Graph n} (C : EdgeColoring c G)
   (hx : P[0]'(by exact List.length_pos_iff.mpr hne) = x)
   (hfree : b ∈ freeColorsOn C x)
   (hnodup : P.Nodup)
+  (ha : a.isSome)
+  (hb : b.isSome)
+  (hneq : a ≠ b)
+
 
 def alternatesColor :=
   alternates (fun v₁ v₂ ↦ color C (v₁, v₂)) a b P
@@ -22,11 +26,16 @@ def alternatesColor :=
 def nextVertex :=
   findNborWithColor C (P.getLast hne) (next a b P)
 
-include hx hfree in
+def lastColor_eq_b_of_nextColor_eq_a :=
+  last_b_of_next_a (fun v₁ v₂ ↦ color C (v₁, v₂)) a b P hne
+
+def lastColor_eq_a_of_nextColor_eq_b :=
+  last_a_of_next_b (fun v₁ v₂ ↦ color C (v₁, v₂)) a b P hne
+
+include hx hfree ha hb hneq in
 theorem nextVertex_not_mem
   (hnodup : P.Nodup)
-
-  (h : (nextVertex C P a b hne).isSome) :
+  (h : (nextVertex C P a b hne).isSome) (hcolor : alternatesColor C P a b) :
   (nextVertex C P a b hne).get h ∉ P := by
   intro hc
   rcases Option.isSome_iff_exists.mp h with ⟨z, hz1⟩
@@ -35,20 +44,66 @@ theorem nextVertex_not_mem
   apply List.find?_some at hz1
   simp at hz1
   rcases List.getElem_of_mem hc with ⟨i, _, hz2⟩
+  subst hz2
   have : i = 0 ∨ 0 < i ∧ i < P.length - 1 ∨ i = P.length - 1 := by
     omega
   rcases this with hi | hi | hi
     -- Case 1: z is the first element
   · subst hi
     rcases next_eq_a_or_b a b P with hnext | hnext
-    · sorry
+    · rw [hnext] at hz1
+      rw [alternatesColor, alternates.eq_def] at hcolor
+      split at hcolor
+      · contradiction
+      · rename_i head hlen
+        simp at hz1
+        rw [self_loop_uncolored C head] at hz1
+        apply Option.ne_none_iff_isSome.mpr at ha
+        exact ha (Eq.symm hz1)
+      · rename_i v₁ v₂ vs hlen
+        simp_all
+        rw [color_symm] at hz1
+        rw [← hcolor.left] at hz1
+        rcases color_unique C _ _ _ hz1 with this | this <;> simp_all
+        have hvs : vs ≠ [] := by
+          by_contra hc
+          subst hc
+          repeat rw [next] at hnext
+          exact hneq (Eq.symm hnext)
+        rw [List.getLast_cons hvs] at this
+        apply List.getLast_mem at hvs
+        simp_all
     · rw [hnext, color_symm] at hz1
-      subst hz2; subst hx
+      subst hx
       apply not_exists_of_freeColor at hfree
       simp_all
     -- Case 2: z is a middle element
-  ·
-    sorry
+  · rw [alternatesColor] at hcolor
+    rcases next_eq_a_or_b a b P with hnext | hnext <;> rw [hnext] at hz1
+    · rcases middle_spec hcolor i hi with ⟨hc, _⟩ | ⟨_, hc⟩
+      · rw [← hz1, color_symm] at ha
+        rw [← hc, color_symm _ _ P[i], color_symm _ _ P[i]] at hz1
+        rcases color_unique C _ _ _ hz1 with this | this <;> simp_all
+        rw [List.getLast_eq_getElem, List.Nodup.getElem_inj_iff hnodup] at this
+        omega
+      · rw [← hz1, color_symm] at ha
+        rw [← hc, color_symm] at hz1
+        rcases color_unique C _ _ _ hz1 with this | this <;> simp_all
+        rw [List.getLast_eq_getElem, List.Nodup.getElem_inj_iff hnodup] at this
+        have := lastColor_eq_b_of_nextColor_eq_a C P a b hne hnext
+        simp_all! +arith
+    · rcases middle_spec hcolor i hi with ⟨_, hc⟩ | ⟨hc, _⟩
+      · rw [← hz1, color_symm] at hb
+        rw [← hc, color_symm] at hz1
+        rcases color_unique C _ _ _ hz1 with this | this <;> simp_all
+        rw [List.getLast_eq_getElem, List.Nodup.getElem_inj_iff hnodup] at this
+        have := lastColor_eq_a_of_nextColor_eq_b C P a b hne hnext
+        simp_all! +arith
+      · rw [← hz1, color_symm] at hb
+        rw [← hc, color_symm _ _ P[i], color_symm _ _ P[i]] at hz1
+        rcases color_unique C _ _ _ hz1 with this | this <;> simp_all
+        rw [List.getLast_eq_getElem, List.Nodup.getElem_inj_iff hnodup] at this
+        omega
     -- Case 3: z is the last element
   · sorry
 
