Vizing/Path/AlternatingPred.lean
@@ -29,6 +29,18 @@ theorem next_eq_a_or_b {V C : Type*} (a b : C) (L : List V) :
   specialize ih b a
   tauto
 
+theorem last_b_of_next_a {V C : Type*} (p : V → V → C) (a b : C) (L : List V) (hne : L ≠ [])
+  (hnext : next a b L = a) : p
+    (L[L.length - 2]'(Nat.sub_lt (List.length_pos_iff.mpr hne) (by omega)))
+    (L[L.length - 1]'(Nat.sub_lt (List.length_pos_iff.mpr hne) (by omega))) = b := by
+    sorry
+
+theorem last_a_of_next_b {V C : Type*} (p : V → V → C) (a b : C) (L : List V) (hne : L ≠ [])
+  (hnext : next a b L = b) : p
+    (L[L.length - 2]'(Nat.sub_lt (List.length_pos_iff.mpr hne) (by omega)))
+    (L[L.length - 1]'(Nat.sub_lt (List.length_pos_iff.mpr hne) (by omega))) = a := by
+    sorry
+
 theorem alternates_concat {V C : Type*} {p : V → V → C} {a b : C} {L : List V} (w : V)
     (Lne : L ≠ [])
     (h : alternates p a b L)
@@ -58,21 +70,48 @@ theorem alternates_tail {V C : Type*} {p : V → V → C} {a b : C} {x : V} {xs 
       subst xs
       exact h.right
 
-theorem middle_spec {V C : Type*} (a b : C) (L : List V) (p : V → V → C)
+theorem alternates_head {V C : Type*} {p : V → V → C} {a b : C} {x : V} {xs : List V}
+    (h : alternates p a b (x :: xs)) (h2 : xs.length > 0) :
+    p x xs[0] = a := by
+    unfold alternates at h
+    split at h <;> rename_i heq
+    · contradiction
+    · simp at heq
+      rcases heq with ⟨_, hc⟩
+      have : xs.length = 0 := by exact List.eq_nil_iff_length_eq_zero.mp hc
+      linarith
+    · simp_all
+
+theorem middle_spec {V C : Type*} {p : V → V → C} {a b : C} {L : List V}
   (h : alternates p a b L)
   (i : Nat) (hi : 0 < i ∧ i < L.length - 1) :
   p L[i-1] L[i] = a ∧ p L[i] L[i+1] = b ∨
   p L[i-1] L[i] = b ∧ p L[i] L[i+1] = a := by
   induction' L with head tail ih generalizing i a b
-  simp at hi
+  · simp at hi
   simp_rw [List.getElem_cons]
   simp_all +arith
-  specialize ih b a (alternates_tail h)
+  specialize @ih b a (alternates_tail h)
   repeat any_goals split
-  linarith
-  · sorry
-  linarith
-  specialize ih (i - 1) (by simp at hi; omega)
-  have : i - 1 + 1 = i := by omega
-  simp_rw [this] at ih
-  tauto
+  · linarith
+  · rename_i h1 h2
+    have htail : tail.length > 0 := by
+      by_contra h
+      simp at h
+      subst h
+      simp at hi
+    have : i = 1 := by omega
+    subst this
+    simp
+    left
+    constructor
+    · exact alternates_head h htail
+    · unfold alternates at h
+      split at h <;> simp_all
+      apply alternates_head h.right
+  · simp_all; omega
+  · specialize ih (i - 1) (by simp_all +arith; omega)
+    have : i - 1 + 1 = i := by omega
+    simp_rw [this] at ih
+    tauto
+
